theories/case_studies/promptcontrol.v
@@ -1,0 +1,280 @@
+From stdpp Require Import base list.
+From iris.proofmode Require Import base tactics.
+From iris.algebra Require Import excl_auth.
+
+
+(* Hazel Reasoning *)
+From hazel.program_logic Require Import weakest_precondition 
+                                        tactics 
+                                        shallow_handler_reasoning 
+                                        deep_handler_reasoning 
+                                        state_reasoning.
+
+(* Local imports *)
+From haffel.lib Require Import base.
+From haffel.lang Require Import haffel.
+From haffel.logic Require Import sem_def.
+From haffel.logic Require Import sem_env.
+From haffel.logic Require Import sem_sig.
+From haffel.logic Require Import sem_row.
+From haffel.logic Require Import sem_types.
+From haffel.logic Require Import ewpw.
+From haffel.logic Require Import sem_judgement.
+From haffel.logic Require Import copyable.
+From haffel.logic Require Import sem_operators.
+From haffel.logic Require Import compatibility.
+From haffel.logic Require Import tactics.
+
+Definition deep_try_alt_ls : val := (
+  rec: "H" "e" "l" "h" "r" :=
+    shallow_try_ls "e" "l" (λ: "x" "k", "H" (λ: <>, "h" "x" "k") "l" "h" "r") "r"
+)%V.
+
+Arguments deep_try_alt_ls : simpl never.
+
+Definition DeepTryAltLS (e : expr) (l : label) (h r : expr) : expr :=
+  deep_try_alt_ls (λ: <>, e)%E (effect l)%V h r.
+
+Definition DeepTryAltLSV (e : expr) (l : label) (h r : expr) : expr :=
+  deep_try_alt_ls (λ: <>, e)%V (effect l)%V h r.
+
+Notation "'deep-try-alt-ls:' e 'handle' l 'with' 'effect' h | 'return' r 'end'" :=
+  (DeepTryAltLS e l h r)
+  (e, l, h, r at level 200, only parsing) : expr_scope.
+
+Definition control : val := (Λ: Λ: λ: "f", perform: (effect "ctrl", "f"))%V.
+Definition controlₘ : val := (Λ: Λ: λ: "f", performₘ: (effect "ctrl", "f"))%V.
+
+Definition prompt : val := 
+  (Λ: λ: "e", 
+    deep-try-alt-ls: "e" #() handle "ctrl" with 
+                effect (λ: "x" "k", "x" "k")
+              | return (λ: "x", "x")
+             end
+  )%V.
+
+Section deep_handler_alt.
+
+  Context `{!heapGS Σ}.
+  
+  Notation deep_handler_alt_ls_type Σ :=
+    (coPset -d> label-d> sem_sig Σ -d> sem_row Σ -d> mode -d> (val -d> iPropO Σ) 
+            -d> expr -d> expr
+            -d> sem_row Σ -d> (val -d> iPropO Σ) -d> iPropO Σ) (only parsing).
+  
+    (* Correctness of the effect branch. *)
+  Definition deep_handler_alt_ls `{irisGS eff_lang Σ} : deep_handler_alt_ls_type Σ := (
+    λ E l σ ρ m Φ h r ρ' Φ',
+    
+    (* Subsumption on row *)
+    (ρ ≤R ρ') ∗
+  
+    (* One-Shot Row *)
+    (⌜ m = OS → OSRow ρ ⌝) ∗
+  
+    (* Correctness of the return branch. *)
+    □?m (
+      ∀ (v : val), Φ v -∗ EWPW r v @ E <| ρ' |> {{ Φ' }}
+    ) ∧
+  
+    (* Correctness of the effect branch. *)
+    □ (
+      ∀ (v k : val),
+        iEff_car (upcl σ.1 σ.2) v (λ w, EWPW k w @ E <| (l, σ) ·: ρ |> {{ Φ }}) -∗
+        EWPW h v k @ E <| (l, σ) ·: ρ |> {{ Φ }}
+    ))%I.
+  
+  Lemma ewpw_deep_try_alt_ls E (l : label) m σ ρ ρ' e (h r : val) Φ Φ' :
+    EWPW e @ E <| (l, σ) ·: ρ |> {{ Φ }} -∗
+    deep_handler_alt_ls E l σ ρ m Φ h r ρ' Φ' -∗
+    EWPW (DeepTryAltLSV e l h r) @E <| ρ' |> {{ Φ' }}.
+  Proof.
+    iIntros "He H". rewrite /DeepTryAltLSV. 
+    iLöb as "IH" forall (e). rewrite /deep_try_alt_ls /ewpw. 
+    rewrite /deep_handler_alt_ls.
+    do 10 ewp_value_or_step. ewp_pure_steps. 
+    iApply (ewpw_shallow_try_ls _ l m  with "He").
+    iDestruct "H" as "(#H1 & %H2 & H3 & #H4)".
+    rewrite /shallow_handler_ls. iFrame "#%".
+    destruct m; simpl.
+    - iSplit; first iApply "H3".
+      iIntros (v k) "(%Φ'' & Hσ & HPost)".
+      rewrite /ewpw; do 6 ewp_value_or_step. 
+      rewrite -/deep_try_alt_ls. iApply ("IH" with "[Hσ HPost]").
+      { iApply "H4". iExists Φ''. iFrame. }
+      iFrame "#%∗".
+    - iDestruct "H3" as "#H3". iIntros "!#".
+      iFrame "#". iIntros (v k) "(%Φ'' & Hσ & HPost)".
+      rewrite /ewpw; do 6 ewp_value_or_step. 
+      rewrite -/deep_try_alt_ls. iApply ("IH" with "[Hσ HPost]").
+      { iApply "H4". iExists Φ''. iFrame. }
+      iFrame "#%∗".
+  Qed.
+  
+  Lemma sem_typed_deep_try_alt_os m l A B τ τ' ρ' ρ'' Γ₁ Γ₂ Γ₃ Γ' x k e h r `{NonExpansive A, NonExpansive B}:
+      x ∉ env_dom Γ₂ → x ∉ env_dom Γ' → x ∉ env_dom Γ₃ → x ∉ env_dom Γ₂ → k ∉ env_dom Γ₂ → k ∉ env_dom Γ₃ → k ∉ env_dom Γ' → x ≠ k →
+      let σ := (∀S: α, A α ⇒ B α | m)%S in
+      let ρ := ((l, σ) ·: ρ')%R in
+      copy_env Γ' -∗
+      ρ' ≤R ρ'' -∗
+      Γ₁ ⊨ e : ρ : τ ⊨ Γ₂ -∗
+      (∀ α, (x, A α) :: (k, B α -{ ρ }-∘ τ) :: Γ' ⊨ h : ρ : τ ⊨ Γ₂) -∗
+      (x, τ) :: Γ₂ ++ Γ' ⊨ r : ρ'' : τ' ⊨ Γ₃ -∗
+      Γ₁ ++ Γ' ⊨ (deep-try-alt-ls: e handle l with
+                          effect  (λ: x k, h)
+                        | return  (λ: x, r) end)%E : ρ'' : τ' ⊨ Γ₃.
+    Proof.
+      iIntros (??????????) "#Hcpy #Hle #He #Hh #Hr !# %vs HΓ₁Γ' /=".
+      iDestruct (env_sem_typed_app with "HΓ₁Γ'") as "[HΓ₁ HΓ'']". 
+      iDestruct ("Hcpy" with "HΓ''") as "#HΓ'". iClear "HΓ''".
+      do 4 ewpw_value_or_step. iDestruct "He" as "-#He".
+      iSpecialize ("He" $! vs with "HΓ₁").
+      iRevert "He". iLöb as "IH" forall (e). iIntros "He".
+      ewpw_pure_steps. 
+      iApply (ewpw_deep_try_alt_ls _ _ MS with "He [HΓ']").
+      rewrite /deep_handler_alt_ls.
+      repeat iSplit; eauto. simpl. iIntros "!#". 
+      - iIntros (v) "[Hτ HΓ₂]". ewpw_pure_steps. rewrite - subst_map_insert. 
+        iApply (ewpw_mono with "[HΓ₂ HΓ' Hτ]").
+        { iApply "Hr". solve_env. iApply env_sem_typed_app; solve_env. }
+        iIntros "!# %w [$ HΓ₃] !>". solve_env.
+      - iIntros (v k') "!# (%Φ & Hρ & HPost)".
+        rewrite sem_sig_eff_eq. iDestruct "Hρ" as "(%α & %a & <- & Ha & Hκb)".
+        ewpw_pure_steps. solve_dec. 
+        rewrite delete_commute - subst_map_insert. 
+        rewrite - delete_insert_ne // - subst_map_insert.
+        iApply (ewpw_mono with "[Hh Ha Hκb HPost]").
+        + iApply "Hh". solve_env. 
+          iSplitL; last (do 2 (rewrite - env_sem_typed_insert; solve_env)).
+          rewrite ! bi.intuitionistically_if_elim.
+          iIntros "% HB". iApply (ewpw_mono with "[HB Hκb HPost]").
+          { iApply "HPost". iApply "Hκb". by iNext. }
+          iIntros "!# % [$ _] //".
+        + iIntros "!# /= % [$ H] !>". do 2 (rewrite - env_sem_typed_insert //).
+    Qed.
+  
+  Lemma sem_typed_deep_try_alt_ms l A B τ τ' ρ' ρ'' Γ₁ Γ₂ Γ₃ Γ' x k e h r `{NonExpansive A, NonExpansive B}:
+      x ∉ env_dom Γ₂ → x ∉ env_dom Γ' → x ∉ env_dom Γ₃ → x ∉ env_dom Γ₂ → k ∉ env_dom Γ₂ → k ∉ env_dom Γ₃ → k ∉ env_dom Γ' → x ≠ k →
+      let σ := (∀S: α, A α ⇒ B α | MS)%S in
+      let ρ := ((l, σ) ·: ρ')%R in
+      copy_env Γ' -∗
+      ρ' ≤R ρ'' -∗
+      Γ₁ ⊨ e : ρ : τ ⊨ Γ₂ -∗
+      (∀ α, (x, A α) :: (k, B α -{ ρ }-> τ) :: Γ' ⊨ h : ρ : τ ⊨ Γ₂) -∗
+      (x, τ) :: Γ₂ ++ Γ' ⊨ r : ρ'' : τ' ⊨ Γ₃ -∗
+      Γ₁ ++ Γ' ⊨ (deep-try-alt-ls: e handle l with
+                          effect  (λ: x k, h)
+                        | return  (λ: x, r) end)%E : ρ'' : τ' ⊨ Γ₃.
+    Proof.
+      iIntros (??????????) "#Hcpy #Hle #He #Hh #Hr !# %vs HΓ₁Γ' /=".
+      iDestruct (env_sem_typed_app with "HΓ₁Γ'") as "[HΓ₁ HΓ'']". 
+      iDestruct ("Hcpy" with "HΓ''") as "#HΓ'". iClear "HΓ''".
+      do 4 ewpw_value_or_step. iDestruct "He" as "-#He".
+      iSpecialize ("He" $! vs with "HΓ₁").
+      iRevert "He". iLöb as "IH" forall (e). iIntros "He".
+      ewpw_pure_steps. 
+      iApply (ewpw_deep_try_alt_ls _ _ MS with "He [HΓ']").
+      rewrite /deep_handler_alt_ls.
+      repeat iSplit; eauto. simpl. iIntros "!#". 
+      - iIntros (v) "[Hτ HΓ₂]". ewpw_pure_steps. rewrite - subst_map_insert. 
+        iApply (ewpw_mono with "[HΓ₂ HΓ' Hτ]").
+        { iApply "Hr". solve_env. iApply env_sem_typed_app; solve_env. }
+        iIntros "!# %w [$ HΓ₃] !>". solve_env.
+      - iIntros (v k') "!# (%Φ & Hρ & HPost)".
+        rewrite sem_sig_eff_eq. iDestruct "Hρ" as "(%α & %a & <- & Ha & Hκb)".
+        ewpw_pure_steps. solve_dec. 
+        rewrite delete_commute - subst_map_insert. 
+        rewrite - delete_insert_ne // - subst_map_insert.
+        iApply (ewpw_mono with "[Hh Ha Hκb HPost]").
+        + iApply "Hh". solve_env; last (do 2 (rewrite - env_sem_typed_insert; solve_env)).
+          iDestruct "Hκb" as "#Hκb". iDestruct "HPost" as "#HPost".
+          iIntros "!# % HB". iApply (ewpw_mono with "[HB Hκb HPost]").
+          { iApply "HPost". iApply "Hκb". by iNext. }
+          iIntros "!# % [$ _] //".
+        + iIntros "!# /= % [$ H] !>". do 2 (rewrite - env_sem_typed_insert //).
+    Qed.
+
+End deep_handler_alt.
+
+Section typing.
+
+  Context `{!heapGS Σ}.
+
+  Definition ctrl_sig (β : sem_ty Σ) (ctrl : sem_row Σ) : label * sem_sig Σ := 
+      ("ctrl", ∀S: α , (α -{ ctrl }-∘ β) -{ ctrl }-∘ β ⇒ α | OS)%S.
+
+  Definition ctrl_pre (β : sem_ty Σ) (ctrl : sem_row Σ) : sem_row Σ := 
+      (ctrl_sig β ctrl ·: ⟨⟩)%R.
+
+  Local Instance contractive_ctrl_pre β : Contractive (ctrl_pre β).
+  Proof.
+    intros ????. rewrite /ctrl_pre. rewrite /sem_row_cons /= /sem_row_ins.
+    intros ?. destruct (decide (i = ("ctrl", 0))) as [->|Hneg].
+    - rewrite !lookup_insert. f_equiv.
+      rewrite /sem_sig_eff. f_equiv. f_equiv. intros ??. 
+      apply non_dep_fun_dist. do 4 f_equiv. f_contractive.
+      apply non_dep_fun_dist. f_equiv; first done. 
+      rewrite /sem_ty_aarr. intros ?. by do 4 f_equiv.
+    - rewrite (lookup_insert_ne _ ("ctrl", 0) i _) //. 
+      rewrite (lookup_insert_ne _ ("ctrl", 0) i _) //.
+  Qed.
+
+  Definition ctrl β : sem_row Σ := (μR: θ, ctrl_pre β θ)%R.
+
+  Local Instance ctrl_sig_ne β θ : NonExpansive (λ α : sem_ty Σ, (α -{ θ }-∘ β) -{ θ}-∘ β).
+  Proof. intros ????. by do 2 f_equiv. Qed.
+
+  Local Instance ctrl_os_row β : OSRow (ctrl β).
+  Proof.
+    rewrite /ctrl. apply row_rec_os_row. iIntros (θ).
+    rewrite /ctrl_pre. apply row_ins_os_row.
+    { rewrite /ctrl_sig. apply sig_eff_os_os_sig; apply _. }
+    simpl. apply row_tun_os_row. apply row_nil_os_row.
+  Qed.
+
+  Definition ctrl_ty : sem_ty Σ := 
+    (∀T: α, ∀T: β, ((α -{ ctrl β }-∘ β) -{ ctrl β }-∘ β) -{ ctrl β }-> α)%T.
+
+  Definition prompt_ty : sem_ty Σ := 
+    (∀T: α, (() -{ ctrl α }-∘ α) → α)%T.
+
+  Lemma ctrl_typed : ⊢ ⊨ᵥ control : ctrl_ty.
+  Proof.
+    iIntros. rewrite /control /ctrl_ty.
+    iApply sem_typed_Tclosure; solve_sidecond. iIntros (α).
+    rewrite - (app_nil_l []).
+    iApply sem_typed_TLam; solve_sidecond. iIntros (β).
+    rewrite - (app_nil_l []).
+    iApply sem_typed_ufun; solve_sidecond. simpl.
+    iApply sem_typed_sub_row; first iApply row_le_rec_fold.
+    rewrite /ctrl_pre -/(ctrl β).
+    iApply (sem_typed_perform_os α _ "ctrl" _ (λ α, α)).
+    iApply sem_typed_var'.
+  Qed.
+
+  Lemma prompt_typed : ⊢ ⊨ᵥ prompt : prompt_ty.
+  Proof.
+    iIntros. rewrite /prompt /prompt_ty.
+    iApply sem_typed_Tclosure; solve_sidecond. iIntros (β).
+    rewrite - (app_nil_l []).
+    iApply sem_typed_ufun; solve_sidecond. simpl.
+    rewrite - (app_nil_r [("e", _)]).
+    set Γ₁ := [("e", () -{ ctrl β }-∘ β)].
+    iApply (sem_typed_deep_try_alt_os OS "ctrl" (λ α, (α -{ ctrl β }-∘ β) -{ ctrl β }-∘ β) (λ α,  α) β β ⟨⟩%R ⟨⟩%R Γ₁ [] [] []); solve_sidecond.  
+    { iApply row_le_nil. }
+    - rewrite /Γ₁. iApply sem_typed_sub_row. 
+      { iApply (row_le_rec_unfold (λ θ, ctrl_pre β θ)). }
+      iApply sem_typed_app_os; last iApply sem_typed_unit'.
+      iApply sem_typed_var'.
+    - iIntros (α). iApply sem_typed_swap_second. 
+      iApply sem_typed_app_os; last iApply sem_typed_var'.
+      iApply sem_typed_sub_nil.
+      iApply sem_typed_sub_ty.
+      + iApply ty_le_aarr; [|iApply ty_le_aarr|]; try iApply ty_le_refl;
+        first iApply (row_le_rec_unfold (λ θ, ctrl_pre β θ)).
+        iApply (row_le_rec_fold (λ θ, ctrl_pre β θ)).
+      + iApply sem_typed_var'.
+    - iApply sem_typed_var.
+  Qed.
+
+End typing.
