theories/case_studies/tossCoin.v
@@ -1,0 +1,55 @@
+From stdpp Require Import base list.
+From iris.proofmode Require Import base tactics.
+From iris.algebra Require Import excl_auth.
+
+
+(* Hazel Reasoning *)
+From hazel.program_logic Require Import weakest_precondition 
+                                        tactics 
+                                        shallow_handler_reasoning 
+                                        deep_handler_reasoning 
+                                        state_reasoning.
+
+(* Local imports *)
+From haffel.lib Require Import base.
+From haffel.lang Require Import haffel.
+From haffel.logic Require Import sem_def.
+From haffel.logic Require Import sem_env.
+From haffel.logic Require Import sem_sig.
+From haffel.logic Require Import sem_row.
+From haffel.logic Require Import sem_types.
+From haffel.logic Require Import sem_judgement.
+From haffel.logic Require Import copyable.
+From haffel.logic Require Import sem_operators.
+From haffel.logic Require Import compatibility.
+From haffel.logic Require Import tactics.
+
+(* The tossCoin example from paper Soundly Hanlding Linearity by Tang et al. *)
+
+Definition tossCoin : val := 
+  (Λ: λ: "g", let: "b" := "g" #() in 
+              if: "b" then #(LitStr "heads") else #(LitStr "tails"))%V.
+
+Section typing.
+
+  Context `{!heapGS Σ}.
+
+  Definition tossCoin_ty : sem_ty Σ := 
+    (∀R: θ, (() -{ θ }-> 𝔹) -{ θ }-> Str)%T.
+
+  Lemma tossCoin_typed : ⊢ ⊨ᵥ tossCoin : tossCoin_ty.
+  Proof.
+    iIntros. rewrite /tossCoin /tossCoin_ty.
+    iApply sem_typed_Rclosure; solve_sidecond. iIntros (θ).
+    rewrite - (app_nil_l []).
+    iApply sem_typed_ufun; solve_sidecond. simpl.
+    iApply (sem_typed_let 𝔹 θ Str _ []); solve_sidecond.
+    - iApply (sem_typed_app_ms ()); solve_sidecond.
+      { iApply sem_typed_sub_ty; first iApply ty_le_u2aarr.
+        iApply sem_typed_var'. }
+      iApply sem_typed_unit'.
+    - iApply sem_typed_if; first iApply sem_typed_var';
+      iApply sem_typed_string'.
+  Qed.
+
+End typing.
